WIP SignatureScheme format

src/tls/Extensions.fst
@@ -45,7 +45,7 @@ noeq
 type extension =
   | E_server_name of list serverName (* M, AF *) (* RFC 6066 *)
   | E_supported_groups of list namedGroup (* M, AF *) (* RFC 7919 *)  
-  | E_signature_algorithms of (list sigHashAlg) (* M, AF *) (* RFC 5246 *)
+  | E_signature_algorithms of signatureSchemes (* M, AF *) (* RFC 5246 *)
   | E_key_share of CommonDH.keyShare (* M, AF *)
   | E_pre_shared_key of (list psk) (* M, AF *)
   | E_early_data of earlyDataIndication
@@ -71,17 +71,17 @@ type extension =
 
 (* string_of_ *)
 let string_of_extension = function
-  | E_server_name _ -> "SNI" 
-  | E_supported_groups _ -> "groups" 
-  | E_signature_algorithms _ -> "sigAlgs"
-  | E_key_share _ -> "keyShare" 
-  | E_pre_shared_key _ -> "PSK"
-  | E_early_data _ -> "EDI"
-  | E_supported_versions _ -> "versions"
+  | E_server_name _ -> "server_name"
+  | E_supported_groups _ -> "supported_groups"
+  | E_signature_algorithms _ -> "signature_algorithms"
+  | E_key_share _ -> "key_share"
+  | E_pre_shared_key _ -> "pre_shared_key"
+  | E_early_data _ -> "early_data"
+  | E_supported_versions _ -> "supported_versions"
   | E_cookie _ -> "cookie"
-  | E_psk_key_exchange_modes _ -> "psk_kex_modes"
+  | E_psk_key_exchange_modes _ -> "psk_key_exchange_modes"
   | E_extended_ms -> "extended_master_secret"
-  | E_ec_point_format _ -> "ec_point_fmt" 
+  | E_ec_point_format _ -> "ec_point_formats"
   | E_unknown_extension (n,_) -> print_bytes n
 
 let rec string_of_extensions = function
@@ -164,7 +164,7 @@ let rec extensionPayloadBytes = function
   | E_server_name []           -> empty_bytes // ServerHello, EncryptedExtensions
   | E_server_name l            -> vlbytes 2 (serverNameBytes l) // ClientHello
   | E_supported_groups l       -> namedGroupsBytes l  
-  | E_signature_algorithms sha -> sigHashAlgsBytes sha
+  | E_signature_algorithms sha -> signatureSchemesBytes sha
   | E_key_share ks             -> CommonDH.keyShareBytes ks
   | E_pre_shared_key psk       -> admit() //PSK.preSharedKeyBytes psk //17-04-21 TODO parse/format the list with ota
   | E_early_data edi           -> earlyDataIndicationBytes edi
@@ -379,7 +379,7 @@ let rec parseExtension role b =
         else Error (AD_decode_error, perror __SOURCE_FILE__ __LINE__ (err_msg "SNI"))
       | (0x00z, 0x0Dz) -> // sigAlgs
         if 2 <= length data && length data < 65538 then
-          (match parseSigHashAlgs data with
+          (match parseSignatureSchemes data with
            | Correct algs -> Correct (E_signature_algorithms algs)
            | Error z -> Error z)
         else Error (AD_decode_error, perror __SOURCE_FILE__ __LINE__ (err_msg "sigAlgs"))
@@ -479,7 +479,7 @@ let rec list_valid_cs_is_list_cs (l:valid_cipher_suites): list cipherSuite =
   | [] -> [] 
   | hd :: tl -> hd :: list_valid_cs_is_list_cs tl
   
-private let rec list_valid_ng_is_list_ng (#p:namedGroup -> Type) (l:list (n:namedGroup{p n})) : list namedGroup = 
+private let rec list_valid_ng_is_list_ng (l:list valid_namedGroup) : list namedGroup = 
   match l with 
   | [] -> [] 
   | hd :: tl -> hd :: list_valid_ng_is_list_ng tl
@@ -507,7 +507,8 @@ val prepareExtensions:
   k:valid_cipher_suites{List.Tot.length k < 256} -> 
   bool -> 
   bool -> 
-  list sigHashAlg -> list (x:namedGroup{SEC? x \/ FFDHE? x}) -> 
+  signatureSchemes -> 
+  list (x:namedGroup{SEC? x \/ FFDHE? x}) -> 
   option (cVerifyData * sVerifyData) ->
   option CommonDH.keyShare -> 
   l:list extension{List.Tot.length l < 256}
@@ -705,28 +706,6 @@ let negotiateClientExtensions pv cfg cExtL sExtL cs ri (resuming:bool) =
        else Error(AD_internal_error, perror __SOURCE_FILE__ __LINE__ "negoClientExts missing extensions in TLS hello message")
      | _ -> Error(AD_internal_error, perror __SOURCE_FILE__ __LINE__ "negoClientExts missing extensions in TLS hello message")
      end 
-     
-(* SI: API. Called by Negotiation. *)
-val clientToNegotiatedExtension: config -> cipherSuite -> option (cVerifyData * sVerifyData) -> bool -> negotiatedExtensions -> extension -> Tot negotiatedExtensions
-let clientToNegotiatedExtension (cfg:config) cs ri resuming neg cExt =
-  match cExt with
-  | E_supported_groups l ->
-      if resuming then neg
-      else
-	  let isOK g = List.Tot.existsb (fun (x:Parse.namedGroup) -> x = g) (list_valid_ng_is_list_ng cfg.namedGroups) in
-	  {neg with ne_supported_groups = Some (List.Tot.filter isOK l)}
-  | E_ec_point_format l ->
-      if resuming then neg
-      else
-	  let nl = List.Tot.filter (fun x -> x = ECGroup.ECP_UNCOMPRESSED) l in
-	  {neg with ne_supported_point_formats = Some nl}
-  | E_server_name l ->
-      {neg with ne_server_names = Some l}
-  | E_signature_algorithms sha ->
-      if resuming then neg
-      else {neg with ne_signature_algorithms = Some (sha)}
-  | _ -> neg // TODO: handle all remaining cases
-
 
 private val clientToServerExtension: protocolVersion -> config -> cipherSuite -> option (cVerifyData * sVerifyData) -> option CommonDH.keyShare -> bool -> extension -> option extension
 let clientToServerExtension pv cfg cs ri ks resuming cext =
@@ -738,31 +717,32 @@ let clientToServerExtension pv cfg cs ri ks resuming cext =
     // See https://tools.ietf.org/html/rfc6066
     match pv, List.Tot.tryFind SNI_DNS? server_name_list with
     | TLS_1p3, _   -> None // TODO: SNI goes in EncryptedExtensions in TLS 1.3
-    | _, Some name -> Some (E_server_name [])
+    | _, Some name -> Some (E_server_name []) // Acknowledge client's choice
+    | _ -> None
     end
   | E_extended_ms -> Some E_extended_ms // REMARK: not depending on cfg.safe_resumption
-  | E_ec_point_format ec_point_format_list ->
+  | E_ec_point_format ec_point_format_list -> // REMARK: ignores client's list
     if resuming || pv = TLS_1p3 then
       None // No ec_point_format in TLS 1.3
     else
       Some (E_ec_point_format [ECGroup.ECP_UNCOMPRESSED])
-  | E_supported_groups named_group_list ->
-    Some (E_supported_groups cfg.namedGroups) // Purely informative
+  | E_supported_groups named_group_list -> // REMARK: Purely informative
+    Some (E_supported_groups (list_valid_ng_is_list_ng cfg.namedGroups)) 
   // TODO: handle all remaining cases
   | E_early_data b -> None
   | E_pre_shared_key b -> None
   | _ -> None
 
-
 (* SI: API. Called by Handshake. *)
-val negotiateServerExtensions: protocolVersion -> option (list extension) -> valid_cipher_suites -> config -> cipherSuite -> option (cVerifyData*sVerifyData) -> option CommonDH.keyShare -> bool -> Tot (result (option (list extension)))
+val negotiateServerExtensions: protocolVersion -> option (list extension) -> valid_cipher_suites -> config -> cipherSuite -> option (cVerifyData * sVerifyData) -> option CommonDH.keyShare -> bool -> result (option (list extension))
 let negotiateServerExtensions pv cExtL csl cfg cs ri ks resuming =
    match cExtL with
    | Some cExtL ->
      let sexts = List.Tot.choose (clientToServerExtension pv cfg cs ri ks resuming) cExtL in
      Correct (Some sexts)
    | None ->
-       (match pv with
+     begin
+     match pv with
 (* SI: deadcode ?
        | SSL_3p0 ->
           let cre =
@@ -771,80 +751,34 @@ let negotiateServerExtensions pv cExtL csl cfg cs ri ks resuming =
               else None //, ne_default in
           in Correct cre
 *)	  
-       | _ -> Error(AD_internal_error, perror __SOURCE_FILE__ __LINE__ "No extensions in ClientHello"))
+     | _ -> 
+       Error(AD_internal_error, perror __SOURCE_FILE__ __LINE__ "No extensions in ClientHello")
+     end
 
-private val default_sigHashAlg_fromSig: protocolVersion -> sigAlg -> ML (list sigHashAlg)
-let default_sigHashAlg_fromSig pv sigAlg=
+// https://tools.ietf.org/html/rfc5246#section-7.4.1.4.1
+private val default_sigHashAlg_fromSig: protocolVersion -> sigAlg ->
+  ML (l:list signatureScheme{List.Tot.length l == 1})
+let default_sigHashAlg_fromSig pv sigAlg =
   let open CoreCrypto in
   let open Hashing.Spec in
   match sigAlg with
-    | RSASIG ->
-        (match pv with
-        | TLS_1p2 -> [(RSASIG, Hash SHA1)]
-        | TLS_1p0 | TLS_1p1 | SSL_3p0 -> [(RSASIG,MD5SHA1)]
-        | TLS_1p3 -> unexpected "[default_sigHashAlg_fromSig] invoked on TLS 1.3")
-        //| SSL_3p0 -> [(RSASIG,NULL)]
-    | DSA ->
-        [(DSA,Hash SHA1)]
-        //match pv with
-        //| TLS_1p0| TLS_1p1 | TLS_1p2 -> [(DSA, SHA1)]
-        //| SSL_3p0 -> [(DSA,NULL)]
-    | _ -> unexpected "[default_sigHashAlg_fromSig] invoked on an invalid signature algorithm"
+  | RSASIG ->
+    begin
+    match pv with
+    | TLS_1p2 -> [ RSA_PKCS1_SHA1 ]
+    | TLS_1p0 | TLS_1p1 | SSL_3p0 -> [ RSA_PKCS1_SHA1 ] // was MD5SHA1
+    | TLS_1p3 -> unexpected "[default_sigHashAlg_fromSig] invoked on TLS 1.3"
+    end
+  | ECDSA -> [ ECDSA_SHA1 ]
+  | _ -> unexpected "[default_sigHashAlg_fromSig] invoked on an invalid signature algorithm"
 
 (* SI: API. Called by HandshakeMessages. *)
-val default_sigHashAlg: protocolVersion -> cipherSuite -> ML (l:list sigHashAlg{List.Tot.length l <= 1})
+val default_sigHashAlg: protocolVersion -> cipherSuite -> ML signatureSchemes
 let default_sigHashAlg pv cs =
   default_sigHashAlg_fromSig pv (sigAlg_of_ciphersuite cs)
 
 
-(*
-let rec (compile_curve_list_aux:list ECGroup.ec_all_curve -> Tot bytes) = function
-  | [] -> empty_bytes
-  | ECGroup.EC_CORE c :: r ->
-    let cid = ECGroup.curve_id c in
-    cid @| compile_curve_list_aux r
-  | ECGroup.EC_EXPLICIT_PRIME :: r -> abyte2 (255z, 01z) @| compile_curve_list_aux r
-  | ECGroup.EC_EXPLICIT_BINARY :: r -> abyte2 (255z, 02z) @| compile_curve_list_aux r
-  | ECGroup.EC_UNKNOWN(x) :: r -> bytes_of_int 2 x @| compile_curve_list_aux r
-
-private val compile_curve_list: l:list ECGroup.ec_all_curve{length (compile_curve_list_aux l) < 65536} -> Tot bytes
-let compile_curve_list l =
-  let al = compile_curve_list_aux l in
-  lemma_repr_bytes_values (length al);
-  let bl: bytes = vlbytes 2 al in
-  bl
-
-val parse_curve_list: bytes -> Tot (result (list ECGroup.ec_all_curve))
-let parse_curve_list b =
-    let rec aux:b:bytes -> Tot (canFail ECGroup.ec_all_curve) (decreases (length b)) = fun b ->
-        if equalBytes b empty_bytes then ExOK([])
-        else if (length b) % 2 = 1 then ExFail(AD_decode_error, perror __SOURCE_FILE__ __LINE__ "Bad encoding of curve list")
-        else
-	  if length b >= 2 then
-	    let (u,v) = split b 2 in
-            (match aux v with
-            | ExFail(x,y) -> ExFail(x,y)
-            | ExOK(l) ->
-                let cur =
-                    (match cbyte2 u with
-                    | (0z, 23z) -> ECGroup.EC_CORE CoreCrypto.ECC_P256
-                    | (0z, 24z) -> ECGroup.EC_CORE CoreCrypto.ECC_P384
-                    | (0z, 25z) -> ECGroup.EC_CORE CoreCrypto.ECC_P521
-                    | (255z, 1z) -> ECGroup.EC_EXPLICIT_PRIME
-                    | (255z, 2z) -> ECGroup.EC_EXPLICIT_BINARY
-                    | _ -> ECGroup.EC_UNKNOWN(int_of_bytes u))
-                in
-                    if List.Tot.mem cur l then ExFail(AD_decode_error, perror __SOURCE_FILE__ __LINE__ "Duplicate curve")
-                    else ExOK(cur :: l))
-	  else ExFail(AD_decode_error, perror __SOURCE_FILE__ __LINE__ "Malformed curve list")
-    in (match aux b with
-    | ExFail(x,y) -> Error(x,y)
-    | ExOK([]) -> Error(AD_decode_error, perror __SOURCE_FILE__ __LINE__ "Empty supported curve list")
-    | ExOK(l) -> correct (l))
-
-(* SI: deadcode
-
-let op_At = FStar.List.Tot.append
+(* Dead code?
 
 val sigHashAlg_contains: list sigHashAlg -> sigHashAlg -> Tot bool
 let sigHashAlg_contains (algList:list sigHashAlg) (alg:sigHashAlg) =
@@ -865,7 +799,7 @@ let rec cert_type_list_to_SigHashAlg ctl pv =
     // FIXME: Generates a list with duplicates!
     match ctl with
     | [] -> []
-    | h::t -> (cert_type_to_SigHashAlg h pv) @ (cert_type_list_to_SigHashAlg t pv)
+    | h::t -> List.Tot.(cert_type_to_SigHashAlg h pv @ cert_type_list_to_SigHashAlg t pv)
 
 val cert_type_to_SigAlg: certType -> Tot sigAlg
 let cert_type_to_SigAlg ct =
@@ -879,38 +813,10 @@ let rec cert_type_list_to_SigAlg ctl =
     match ctl with
     | [] -> []
     | h::t -> (cert_type_to_SigAlg h) :: (cert_type_list_to_SigAlg t)
+
+val cert_type_to_SigHashAlg: certType -> protocolVersion -> list sigHashAlg
+let cert_type_to_SigHashAlg ct pv =
+    match ct with
+    | TLSConstants.DSA_fixed_dh | TLSConstants.DSA_sign -> default_sigHashAlg_fromSig pv DSA
+    | TLSConstants.RSA_fixed_dh | TLSConstants.RSA_sign -> default_sigHashAlg_fromSig pv RSASIG
 *)
-
-(* val sigHashAlg_contains: list sigHashAlg -> sigHashAlg -> Tot bool *)
-(* let sigHashAlg_contains (algList:list sigHashAlg) (alg:sigHashAlg) = *)
-(*     List.Tot.mem alg algList *)
-
-(* val sigHashAlg_bySigList: list sigHashAlg -> list sigAlg -> Tot (list sigHashAlg) *)
-(* let sigHashAlg_bySigList (algList:list sigHashAlg) (sigAlgList:list sigAlg) = *)
-(*     List.Tot.choose (fun alg -> let (sigA,_) = alg in if (List.Tot.existsb (fun a -> a = sigA) sigAlgList) then Some(alg) else None) algList *)
-
-(* val cert_type_to_SigHashAlg: certType -> protocolVersion -> list sigHashAlg *)
-(* let cert_type_to_SigHashAlg ct pv = *)
-(*     match ct with *)
-(*     | TLSConstants.DSA_fixed_dh | TLSConstants.DSA_sign -> default_sigHashAlg_fromSig pv DSA *)
-(*     | TLSConstants.RSA_fixed_dh | TLSConstants.RSA_sign -> default_sigHashAlg_fromSig pv RSASIG *)
-
-(* val cert_type_list_to_SigHashAlg: list certType -> protocolVersion -> list sigHashAlg *)
-(* let rec cert_type_list_to_SigHashAlg ctl pv = *)
-(*     // FIXME: Generates a list with duplicates! *)
-(*     match ctl with *)
-(*     | [] -> [] *)
-(*     | h::t -> (cert_type_to_SigHashAlg h pv) @ (cert_type_list_to_SigHashAlg t pv) *)
-
-(* val cert_type_to_SigAlg: certType -> Tot sigAlg *)
-(* let cert_type_to_SigAlg ct = *)
-(*     match ct with *)
-(*     | TLSConstants.DSA_fixed_dh | TLSConstants.DSA_sign -> DSA *)
-(*     | TLSConstants.RSA_fixed_dh | TLSConstants.RSA_sign -> RSASIG *)
-
-(* val cert_type_list_to_SigAlg: list certType -> list sigAlg *)
-(* let rec cert_type_list_to_SigAlg ctl = *)
-(*     // FIXME: Generates a list with duplicates! *)
-(*     match ctl with *)
-(*     | [] -> [] *)
-(*     | h::t -> (cert_type_to_SigAlg h) :: (cert_type_list_to_SigAlg t) *)
